
\documentclass[../Main/main]{subfiles}


\begin{document}


\unit{ $ New $ }
{
	
	\proposition{ $  $ }
	{
		\letbe
		{
			|\lambda| < 1 < |\mu|
		}
		\holds
		{
			A^n = \lambda^n, \mu^n.
			\all{ (x,y) \in \R^2 }[ y \neq 0 ]
			{
				o((x,y)) \convergesto (0,\infty)
			}.
			\all{ (x,y) \in \R^2 }[ y = 0 ]
			{
				o((x,y)) \convergesto (0,0)
			}
		}
		\demonstration
		{
			x_n = \lambda^n x \convergesto 0.
			y_n = \mu^n y \convergesto \begin{cases} 0 & y = 0 \\ \infty & y \neq 0 \end{cases} 
		}
	}
	
	
	\definition{ $ Stable \& Unstable subspaces $ }
	{
		\letbe
		{
			A \in \Mc_{2\times 2}(\R)
		}
		\name{ $ stable subspace of $ A	}
		{
			
		}
		\name{ $ unstable subspace of $ A }
		{

		}
		\denote
		{
			E^s, E^u
		}
	}


	\proposition{ $ abstract $ }
	{
		\letbe
		{
			A = \lambda, 1 \lambda, 0
		}
		\holds
		{
			\abs{ \lambda } < 1 \imp o(x,y)\convergesto (0,0).
			\abs{ \lambda } > 1 \imp o(x,y)\convergesto (\infty,\infty)			
		}
		\demonstration
		{
			A^n = \lambda^{n-1}( \lambda, n, 0, \lambda ).
		}
	}
	
	
	\proposition{ $ Origin stability theorem $ }
	{
		\letbe
		{
			A \in \Mc_{n\times n}(\R).
			\definedFunction{ f }{ \R^n }{ \R^n }{ x }{ Ax }.
			\sigma(A) $ eigenvalues of $ A
		}
		\holds
		{
			\all{ i \in \indexes{ 1 }{ n } }
			{
				\abs{ \lambda_i } < 1
			} \imp $ origin is attractive $.

			\all{ i \in \indexes{ 1 }{ n } }
			{
				\abs{ \lambda_i } > 1
			} \imp $ origin is repulsive $.
			\ex{ \lambda_1,\lambda_2 \in \sigma(A) }
			{
				\abs{ \lambda_1 } > 1 \logicAnd \abs{ \lambda_2 } < 1 
			} \imp \R^n = E^s + E^u
		}
		\demonstration
		{
			demonstration.
		}
	}
	
	
	\proposition{ $ Local stability of fixed points of non-linear applications $ }
	{
		\letbe
		{
			\function{ f }{ \R^n }{ \R^n }.
			x \in \fixed( f ).
			\Uc \subset \R^n $ open $ \suchthat x \in \Uc
			\function{ f }{ \Uc }{ \R^n } $ differentiable in $ x
		}
		\holds
		{
			\rho( Df(p) ) < 1 \imp x $ attractive $.
			\all{ \lambda \in \sigma(A) }
			{
				\abs{ \lambda } > 1
			} \imp x $ repulsive $ 
		}
		\demonstration
		{
			$Suppose $ p = 0.

			\be{ A }{ Df(0) }.

			$Consider:$.

			\function{ ||-|| }{ \R^n }{ \R^n } $ norm $ \suchthat ||A|| < 1.

			
			\ex{ \Uc \subset \R^n $ open $ }
			{
				f \in \Cc^1(\Uc)
				\all{ v \in \R^n }
				{
					f(v) = Av + \mu(v) \suchthat \limit{ \frac{ \mu(v) }{ ||v|| } }{ v }[ 0 ] = 0
				}
			}.

			\all{ \eta \in \R^+ }
			{
				\ex{ r \in \R^+ }
				{
					||v|| < r \imp ||\mu(v)|| \leq \eta||v||
				}
			}
			\be{ \eta }{ a+\eta < 1 }.

			\all{ n \in \N }
			{
				\all{ v \in \D(0,r) }
				{
					f^n(v) \in \D(0,r).
					||f^n(v)|| \leq (a + \eta)^n||v||
				}
			}

			\induction{ n }
			{
				n = 0 $ ok $.

				$Suppose true for $ n.

				||f^{n+1}(v)|| = ||f(f^n(v))|| \leq ||Af^n(v)|| + ||\mu(f^n(v))||.
				\leq a||f^n(v)|| + \eta||f^n(v)|| = (a + \eta) ||f^n(v)|| \leq (a+\eta)^{n+1} ||v||


			}.

			\all{ \epsilon \in \R^+ }
			{
				\be{ \delta }{ \min(\epsilon,r) }.

				\all{ v \in \R^n }[ ||v|| < \delta ]
				{
					||f^n(v)|| \leq (a + \eta)^n||v|| \leq ||v|| < \epsilon.

					||f^n(v)|| \convergesto 0
				}
			}.



			$repulsive:$.

			D(f^{-1})(x) = (Df(x))^{-1}.
			\be{ A }{ D(f^{-1})(x) }.

			A^{-1} = (Df(x))^{-1}.

			\sigma(A^{-1}) = \sigma(A)^{-1}.

			x $ attractive by $ f^{-1} \imp x $ repulsive by $ f
		}
	}
	
	
	\proposition{ $ Local stability of periodic points $ }
	{
		\letbe
		{
			\function{ f }{ \R^n }{ \R^n }.
			x \in \R^n $ period $ k $ point $.
			o(x) $ orbit of $ x
		}
		\holds
		{
			\all{ p_i \in o(x) }
			{
				\be{ A_i }{ Df^k(p_i) = Df(p_{i-1})---Df(p_k)---Df(p_i)}.

				\sigma(A_i) = \sigma(A_{i'})
			}
		}
		\demonstration
		{
			$ regla de la cadena da producto de matrices que no es conmutativo $
		}
	}
	
	
	\definition{ $ Invariant stable \& unstable manifold $ }
	{
		\letbe
		{
			\function{ f }{ \R^n }{ \R^n }
		}
		\name{ $ invariant stable manifold of $ x }
		{
			\set{ v \in \R^n \with f^n \convergesto 0 }
		}
		\name{ $ invariant unstable manifold of $ x }
		{
			\set{ v \in \R^n \with f^{-n} \convergesto 0 }
		}
		\denote
		{
			$stable invariant manifold $ \as W^s.
			$unstable invariant manifold $ \as W^u
		}
	}
	
	
	\example{ $ Stable \& unstable invariant manifolds $ }
	{
		\letbe
		{
			\definedFunction{ f }{ \R^2 }{ \R^2 }{ (x,y) }{ (\frac{ x }{ 2 }, 2y - 7x^2) }
		}
		\study
		{
			$stability of $ \fixed( f )
		}
		\start
		{
			Df(x,y) = \Matrix{ 1/2,0.-4x,2 }.

			Df(0,0) = \Matrix{ 1/2,0.0,2 }.

			\sigma(Df(0,0)) = \set{ 1/2, 2 } \imp (0,0) $ sella point $.

			\all{ y \in \R }
			{
				f(0,y) = (0,2y) \imp f^n(0,y) = (0,2^n) \convergesto \infty.

				\set{ (x,y) \in \R^2 \with x = 0 } \subset W^u(0,0)
			}.

			\be{ C }{ \set{ (x,y) \in \R^2 \with y = 4x^2 } }.

			\all{ (x,y) \in C }
			{
				f(x,y) = f(x,4x) = ( x/2, x^2 ) \in C.
				f^{-1}(x,y) = (2x,16x^2) \in C.
				f^n(x,4x) = (x/2^n, x^2/2^{2n-2}) \convergesto (0,0)
			}.

			W^s(0,0) = C
		}	
	}
	
	
	\proposition{ $ Stable manifold theorem $ }
	{
		\letbe
		{
			\Uc \subset \R^n $ open $.
			\function{ f }{ \Uc }{ \R^n } \in \Cc^r(\Uc).
			p \in \R^2 $ sella fixed point $
		}
		\holds
		{
			\ex{ \function{ \gamma }{ [a,b] }{ \R^2 } \in \Cc^r([a,b]) }
			{
				\gamma(0) = p.
				\gamma'(0) \neq 0.

				\all{ i \in \indexes{ 1 }{ r } }
				{
					Df^r(p) = \gamma^r(0)
				}

				W^s(p) $ tangent $ W^s(p).
				W^u(p) $ tangent $ E^u(p)
			}
		}
		\demonstration
		{
			$ no demonstration $
		}
	}
	
	
	\example{ $ 45. Stability of periodic points $ }
	{
		\letbe
		{
			\definedFunction{ f }{ \R^2 }{ \R^2 }{ (x,y) }{ (2x+y^2 - 2, x^2 -x -y^3) }
		}
		\study
		{
			$Stability of $ \fixed( f )
		}
		\start
		{
			f(1,1) = (2+1-2,1-1-1) = (1,-1).

			f(1,-1) = (2+1-2,1-1+1) = (1,1).

			(1,1) $ period $ 2 $ point $.

			Df(x,y) = \Matrix{ 2,2y. 2x-1,-3y^2 }.

			Df^2(1,1) = \Matrix{ 2,10,-1,11 } \neq Df^2(1,-1).

			\chi_A(t) = t^2 - 13t + 32.

			\sigma(A) = \set{ 3,29---, 9,70--- }.

			\all{ \lambda \in \sigma(A) }
			{
				\abs{ \lambda } > 1
			}.

			$Stability theorem$:

			(1,1) $ repulsive $
		}
	}
	
	
	\example{ $ 46. Explicit solution of non-linear applications $ }
	{
		\letbe
		{
			\definedFunction{ f }{ \R^2 }{ \R^2 }{ (x,y) }{ (2x-y^3,1/2y) }
		}
		\holds
		{
			\Matrix{ 2x-y = t. 1/2y = s } $ determinated system $ \imp f $ inyective $.

			$Suppose$ (x_{n+1},y_{n+1}) = (2^n(2x_0-y_0^3 - ... - \frac{ 1 }{ 4^{2n} }y_0^3), \frac{ 1 }{ 2^{n+1} }y_0).

			\induction{ n }
			{
				n = 1.

				(x_1,y_1) = (2^0(2x_0-y_0^3), 1/2 y^0) $ok$.

				\all{ n \in \N }
				{
					$ Suppose true for $ n.

					(x_{n+1},y_{n+1}) = f(x_n,y_n) $ok$
				}
			}..

			\be{ C }{ \set{ (x,y) \in \R^2 \with x = \frac{ 8 }{ 15 }y^3 } }.

			c $ stable manifold of the origin $.

			\all{ (x,y) \in C }
			{
				\all{ n \in \N }
				{
					(x_n,y_n) \in C.
					$calculus----$.
				}.

				o(x,y) \convergesto (0,0).

				y_{n+1} = \frac{ 1 }{ 2^{n+1} }y_0 \convergesto 0.

				x_{n+1} = \frac{ 8 }{ 15 }y_{n+1}^3 \convergesto 0.

			}

			f $ inyective $ \imp \all{ (x,y) \in \C }
			{
				f^{-1}(x,y) \in C
			}.

			C $ is The invariant manifold over the origin $
		}
	}
	

	\definition{ $ Contractive application $ }
	{
		\letbe
		{
			statements.
		}
		\then{ item }{ $ a/an entity $ }
		{
			conditions.
		}
		\denote
		{
			property \as notation.
		}
	}
	
	
	
	
	\proposition{ $ Fixed point theorem $ }
	{
		\letbe
		{
			\Uc \subset \R^n $ closed $.
			\function{ f }{ \Uc }{ \Uc } \lambda-$contractive$
		}
		\holds
		{
			\fixed( f ) = \{ p \}.
			p $ global attractive fixed point $.
			a.
			b		
		}
		\demonstration
		{
			\all{ x \in \Uc }
			{
				\be{ x_n }{ f^n(x) }
			}.

			f $ contractive $ \imp ||x_n - y_n|| \leq \lambda^n||x_0-y_0||.

			$In particular:$.

			y = f(x) = x_1 \imp ||x_n - x_{n+1}|| \leq \lambda^n||x_0-x_1||.

			\sequence{ x_n }{ n } $ Cauchy sequence $.

			\sequence{ x_n }{ n } \subset \R^n, \R^n $ complete $ \imp \sequence{ x_n }{ n } $ convergent $.

			f $ contractive $ \imp f $ continuous$.

			f(p) = f(\limit{ x_n }{ n }) = \limit{ f(x_n) }{ n } = \limit{ x_{n+1} }{ n } = p.

			p $ fixed point $.

			\all{ p,q \in \Uc }[ p,q $ fixed points $ ]
			{
				||f^n(p) - f^n(q)|| \leq \lambda^n||p-q|| \convergesto 0.

				||p-q|| \convergesto 0.

				$absurd$
			}.

			\all{ x \in \R^n }
			{
				||f^n(x) - p || = ||f^n(x)-f^n(p)|| \leq \lambda^n||x-p|| \convergesto 0
			}
		}
	}
	
	
	
	
	
	
	
	
}


\end{document}